Use new bytes type

SerializerRewrite.v
@@ -11,41 +11,60 @@ Arguments Done {_} {_} _.
 Arguments More {_} {_} _.
 Arguments Error {_} {_}.
 
+Inductive byte :=
+| x00 | x01 | x02 | x03 | x04 | x05 | x06 | x07 | x08 | x09 | x0a | x0b | x0c
+| x0d | x0e | x0f | x10 | x11 | x12 | x13 | x14 | x15 | x16 | x17 | x18 | x19
+| x1a | x1b | x1c | x1d | x1e | x1f | x20 | x21 | x22 | x23 | x24 | x25 | x26 
+| x27 | x28 | x29 | x2a | x2b | x2c | x2d | x2e | x2f | x30 | x31 | x32 | x33 
+| x34 | x35 | x36 | x37 | x38 | x39 | x3a | x3b | x3c | x3d | x3e | x3f | x40 
+| x41 | x42 | x43 | x44 | x45 | x46 | x47 | x48 | x49 | x4a | x4b | x4c | x4d 
+| x4e | x4f | x50 | x51 | x52 | x53 | x54 | x55 | x56 | x57 | x58 | x59 | x5a 
+| x5b | x5c | x5d | x5e | x5f | x60 | x61 | x62 | x63 | x64 | x65 | x66 | x67 
+| x68 | x69 | x6a | x6b | x6c | x6d | x6e | x6f | x70 | x71 | x72 | x73 | x74 
+| x75 | x76 | x77 | x78 | x79 | x7a | x7b | x7c | x7d | x7e | x7f | x80 | x81 
+| x82 | x83 | x84 | x85 | x86 | x87 | x88 | x89 | x8a | x8b | x8c | x8d | x8e 
+| x8f | x90 | x91 | x92 | x93 | x94 | x95 | x96 | x97 | x98 | x99 | x9a | x9b 
+| x9c | x9d | x9e | x9f | xa0 | xa1 | xa2 | xa3 | xa4 | xa5 | xa6 | xa7 | xa8 
+| xa9 | xaa | xab | xac | xad | xae | xaf | xb0 | xb1 | xb2 | xb3 | xb4 | xb5 
+| xb6 | xb7 | xb8 | xb9 | xba | xbb | xbc | xbd | xbe | xbf | xc0 | xc1 | xc2 
+| xc3 | xc4 | xc5 | xc6 | xc7 | xc8 | xc9 | xca | xcb | xcc | xcd | xce | xcf 
+| xd0 | xd1 | xd2 | xd3 | xd4 | xd5 | xd6 | xd7 | xd8 | xd9 | xda | xdb | xdc 
+| xdd | xde | xdf | xe0 | xe1 | xe2 | xe3 | xe4 | xe5 | xe6 | xe7 | xe8 | xe9 
+| xea | xeb | xec | xed | xee | xef | xf0 | xf1 | xf2 | xf3 | xf4 | xf5 | xf6 
+| xf7 | xf8 | xf9 | xfa | xfb | xfc | xfd | xfe | xff.
+
 Definition leastBit (a : ascii) :=
   match a with
   | Ascii b _ _ _ _ _ _ _ => b
   end.          
 
-Definition ascii_eq a b :=
-  if ascii_dec a b then true else false.
-           
 Module Type SERIALIZER.
   Parameter t : Type.
   Parameter empty : t.
   Parameter append : t -> t -> t.
-  Parameter putByte : ascii -> t.
+  Parameter putByte : byte -> t.
 
   (* For proof only! Do not call from serializers. *)
-  Parameter unwrap : t -> list ascii.
+  Parameter unwrap : t -> list byte.
   Parameter empty_unwrap : unwrap empty = [].
   Parameter append_unwrap :
       forall x y : t, unwrap (append x y) = unwrap x ++ unwrap y.
-  Parameter putByte_unwrap : forall (a : ascii), unwrap (putByte a) = [a].
+  Parameter putByte_unwrap : forall (a : byte), unwrap (putByte a) = [a].
 End SERIALIZER.
 
 Module Serializer : SERIALIZER.
-  Definition t := list ascii.
+  Definition t := list byte.
   Definition empty : t := [].
-  Definition putByte (a : ascii) : t := [a].
+  Definition putByte (a : byte) : t := [a].
 
   Definition append (x y : t) : t := x ++ y.
 
-  Definition unwrap (x : t) : list ascii := x.
+  Definition unwrap (x : t) : list byte := x.
 
   Lemma empty_unwrap : unwrap empty = [].
   Proof. reflexivity. Qed.
 
-  Lemma putByte_unwrap : forall (a : ascii), unwrap (putByte a) = [a].
+  Lemma putByte_unwrap : forall (a : byte), unwrap (putByte a) = [a].
   Proof. reflexivity. Qed.
 
   Lemma append_unwrap :
@@ -56,8 +75,8 @@ End Serializer.
 Module Type DESERIALIZER.
   Parameter t : Type -> Type.
 
-  Parameter getByte : t ascii.
-  Parameter unwrap : forall A, t A -> list ascii -> option (A * list ascii).
+  Parameter getByte : t byte.
+  Parameter unwrap : forall A, t A -> list byte -> option (A * list byte).
 
   Parameter getByte_unwrap : forall l,
       unwrap getByte l = match l with
@@ -67,10 +86,11 @@ Module Type DESERIALIZER.
 
   Parameter bind : forall A B, t A -> (A -> t B) -> t B.
   Parameter ret : forall A, A -> t A.
+  Parameter fail : forall A, t A.
   Parameter map : forall A B, (A -> B) -> t A -> t B.
 
   Parameter fold : forall S A,
-      (ascii -> S -> fold_state S A) -> S -> t A.
+      (byte -> S -> fold_state S A) -> S -> t A.
 
   Parameter bind_unwrap : forall A B (m : t A)
                              (f : A -> t B) bytes,
@@ -87,7 +107,7 @@ Module Type DESERIALIZER.
       end.
 
   Parameter fold_unwrap : forall {S A : Type}
-                             (f : ascii -> S -> fold_state S A) (s : S) l,
+                             (f : byte -> S -> fold_state S A) (s : S) l,
       unwrap (fold f s) l =
       match l with
       | [] => None
@@ -100,10 +120,10 @@ Module Type DESERIALIZER.
 End DESERIALIZER.
 
 Module Deserializer : DESERIALIZER.
-  Definition t (A : Type) := list ascii -> option (A * list ascii).
+  Definition t (A : Type) := list byte -> option (A * list byte).
   Definition unwrap {A} (x : t A) := x.
 
-  Definition getByte (l : list ascii) :=
+  Definition getByte (l : list byte) :=
     match l with
     | [] => None
     | b :: l => Some (b, l)
@@ -119,6 +139,9 @@ Module Deserializer : DESERIALIZER.
   Definition ret {A} (a : A) : t A :=
     fun l => Some (a, l).
 
+  Definition fail {A} : t A :=
+    fun l => None.
+  
   Definition map {A B} (f : A -> B) (d : t A) : t B :=
     bind d (fun a => ret (f a)).
 
@@ -142,7 +165,7 @@ Module Deserializer : DESERIALIZER.
   Qed.
 
   Fixpoint fold {S A}
-           (f : ascii -> S -> fold_state S A) (s : S) (l : list ascii) :=
+           (f : byte -> S -> fold_state S A) (s : S) (l : list byte) :=
     match l with
     | [] => None
     | b :: l => match f b s with
@@ -164,7 +187,7 @@ Module Deserializer : DESERIALIZER.
   Proof. reflexivity. Qed.
 
   Lemma fold_unwrap : forall {S A : Type}
-                             (f : ascii -> S -> fold_state S A) (s : S) l,
+                             (f : byte -> S -> fold_state S A) (s : S) l,
       unwrap (fold f s) l =
       match l with
       | [] => None
@@ -179,7 +202,8 @@ Module Deserializer : DESERIALIZER.
     simpl. destruct l; reflexivity.
   Qed.
 End Deserializer.
-
+Arguments Deserializer.fail {_}.
+          
 Notation serialize_deserialize_id_spec s d :=
   (forall a bin,
       Deserializer.unwrap d (Serializer.unwrap (s a) ++ bin) = Some(a, bin)).
@@ -216,7 +240,7 @@ Lemma serialize_deserialize_ascii_id :
   serialize_deserialize_id_spec Serializer.putByte Deserializer.getByte.
 Proof. cheerios_crush. Qed.
 
-Instance ascii_Serializer : Serializer ascii :=
+Instance byte_Serializer : Serializer byte :=
   {| serialize := Serializer.putByte;
      deserialize := Deserializer.getByte;
      serialize_deserialize_id := serialize_deserialize_ascii_id |}.
@@ -225,8 +249,8 @@ Instance ascii_Serializer : Serializer ascii :=
 
 Lemma fold_append_unwrap :
   forall {S A : Type}
-         (f : ascii -> S -> fold_state S A) (s : S)
-         (b : ascii) (tail : Serializer.t) (bin : list ascii),
+         (f : byte -> S -> fold_state S A) (s : S)
+         (b : byte) (tail : Serializer.t) (bin : list byte),
     Deserializer.unwrap (Deserializer.fold f s)
                         (Serializer.unwrap (Serializer.append
                                               (serialize b)
@@ -243,8 +267,8 @@ Qed.
 
 Lemma fold_append_unwrap' :
   forall {S A : Type}
-         (f : ascii -> S -> fold_state S A) (s : S)
-         (b : ascii) (tail : Serializer.t) (bin : list ascii),
+         (f : byte -> S -> fold_state S A) (s : S)
+         (b : byte) (tail : Serializer.t) (bin : list byte),
     Deserializer.unwrap (Deserializer.fold f s)
                         (Serializer.unwrap (Serializer.append
                                               (Serializer.putByte b)
@@ -309,74 +333,61 @@ Local Open Scope char_scope.
 
 Fixpoint serialize_positive p :=
   match p with
-  | xI (xI (xI p)) => Serializer.append (serialize "014")
+  | xI (xI (xI p)) => Serializer.append (serialize x0e)
                                         (serialize_positive p)
-  | xI (xI (xO p)) => Serializer.append (serialize "013")
+  | xI (xI (xO p)) => Serializer.append (serialize x0d)
                                         (serialize_positive p)
-  | xI (xO (xI p)) => Serializer.append (serialize "012")
+  | xI (xO (xI p)) => Serializer.append (serialize x0c)
                                         (serialize_positive p)
-  | xI (xO (xO p)) => Serializer.append (serialize "011")
+  | xI (xO (xO p)) => Serializer.append (serialize x0b)
                                         (serialize_positive p)
-  | xO (xI (xI p)) => Serializer.append (serialize "010")
+  | xO (xI (xI p)) => Serializer.append (serialize x0a)
                                         (serialize_positive p)
-  | xO (xI (xO p)) => Serializer.append (serialize "009")
+  | xO (xI (xO p)) => Serializer.append (serialize x09)
                                         (serialize_positive p)
-  | xO (xO (xI p)) => Serializer.append (serialize "008")
+  | xO (xO (xI p)) => Serializer.append (serialize x08)
                                         (serialize_positive p)
-  | xO (xO (xO p)) => Serializer.append (serialize "007")
+  | xO (xO (xO p)) => Serializer.append (serialize x07)
                                         (serialize_positive p)
-  | xI (xI p) => Serializer.append (serialize "006")
+  | xI (xI p) => Serializer.append (serialize x06)
                                    (serialize_positive p)
-  | xI (xO p) => Serializer.append (serialize "005")
+  | xI (xO p) => Serializer.append (serialize x05)
                                    (serialize_positive p)
-  | xO (xI p) => Serializer.append (serialize "004")
+  | xO (xI p) => Serializer.append (serialize x04)
                                    (serialize_positive p)
-  | xO (xO p) => Serializer.append (serialize "003")
+  | xO (xO p) => Serializer.append (serialize x03)
                                    (serialize_positive p)
-  | xI p => Serializer.append (serialize "002")
+  | xI p => Serializer.append (serialize x02)
                               (serialize_positive p)
-  | xO p => Serializer.append (serialize "001")
+  | xO p => Serializer.append (serialize x01)
                               (serialize_positive p)
-  | XH => serialize "000"
+  | XH => serialize x00
   end.
 
 Definition deserialize_positive_step
-           (b : ascii)
+           (b : byte)
            (s : positive -> positive) := 
-  if ascii_eq b "014"
-  then More (fun p => s (xI (xI (xI p))))
-  else if ascii_eq b "013"
-       then More (fun p => s (xI (xI (xO p))))
-       else if ascii_eq b "012"
-            then More (fun p => s (xI (xO (xI p))))
-            else if ascii_eq b "011"
-                 then More (fun p => s (xI (xO (xO p))))
-                 else if ascii_eq b "010"
-                      then More (fun p => s (xO (xI (xI p))))
-                      else if ascii_eq b "009"
-                           then More (fun p => s (xO (xI (xO p))))
-                           else if ascii_eq b "008"
-                                then More (fun p => s (xO (xO (xI p))))
-                                else if ascii_eq b "007"
-                                     then More (fun p => s (xO (xO (xO p))))
-                                     else if ascii_eq b "006"
-                                          then More (fun p => s (xI (xI p)))
-                                          else if ascii_eq b "005"
-                                               then More (fun p => s (xI (xO p)))
-                                               else if ascii_eq b "004"
-                                                    then More (fun p => s (xO (xI p)))
-                                                    else if ascii_eq b "003"
-                                                         then More (fun p => s (xO (xO p)))
-                                                         else if ascii_eq b "002"
-                                                              then More (fun p => s (xI p))
-                                                              else if ascii_eq b "001"
-                                                                   then More (fun p => s (xO p))
-                                                                   else if ascii_eq b "000"
-                                                                        then Done (s xH)
-                                                                        else Error.
+  match b with
+  | x0e => More (fun p => s (xI (xI (xI p))))
+  | x0d => More (fun p => s (xI (xI (xO p))))
+  | x0c => More (fun p => s (xI (xO (xI p))))
+  | x0b => More (fun p => s (xI (xO (xO p))))
+  | x0a => More (fun p => s (xO (xI (xI p))))
+  | x09 => More (fun p => s (xO (xI (xO p))))
+  | x08 => More (fun p =>  s (xO (xO (xI p))))
+  | x07 => More (fun p => s (xO (xO (xO p))))
+  | x06 => More (fun p => s (xI (xI p)))
+  | x05 => More (fun p => s (xI (xO p)))
+  | x04 => More (fun p => s (xO (xI p)))
+  | x03 => More (fun p => s (xO (xO p)))
+  | x02 => More (fun p => s (xI p))
+  | x01 => More (fun p => s (xO p))
+  | x00 => Done (s xH)
+  | _ => Error
+  end.
 
 Definition positive_step_aux p :=
-  forall (k : positive -> positive) (bytes : list ascii),
+  forall (k : positive -> positive) (bytes : list byte),
     Deserializer.unwrap (Deserializer.fold deserialize_positive_step k)
                         (Serializer.unwrap (serialize_positive p) ++ bytes)
     = Some(k p, bytes).
@@ -420,15 +431,17 @@ Qed.
 
 Definition serialize_N n :=
   match n with
-  | N0 => serialize zero
-  | Npos p => Serializer.append (serialize one) (serialize p)
+  | N0 => serialize x00
+  | Npos p => Serializer.append (serialize x01) (serialize p)
   end.
 
 Definition deserialize_N :=
   Deserializer.bind deserialize
-                    (fun (b : ascii) => if leastBit b
-                                       then Deserializer.map Npos deserialize
-                                       else Deserializer.ret N0).
+                    (fun (b : byte) => match b with
+                                       | x00 => Deserializer.ret N0
+                                       | x01 => Deserializer.map Npos deserialize
+                                       | _ => Deserializer.fail
+                                       end).
 
 Theorem serialize_deserialize_N_id :
   serialize_deserialize_id_spec serialize_N deserialize_N.
@@ -501,16 +514,18 @@ Section combinators.
   
   Definition option_serialize (x : option A) : Serializer.t :=
     match x with
-    | Some a => Serializer.append (serialize one) (serialize a)
-    | None => serialize zero
+    | Some a => Serializer.append (serialize x01) (serialize a)
+    | None => serialize x00
     end.
 
   Definition option_deserialize : Deserializer.t (option A) :=
     Deserializer.bind deserialize
-                      (fun (b : ascii) =>
-                         if leastBit b
-                         then Deserializer.map (@Some A) deserialize
-                         else Deserializer.ret None).
+                      (fun (b : byte) =>
+                         match b with
+                         | x01 => Deserializer.map (@Some A) deserialize
+                         | x00 => Deserializer.ret None
+                         | _ => Deserializer.fail
+                         end).
 
   Lemma serialize_deserialize_option :
     serialize_deserialize_id_spec option_serialize option_deserialize.
@@ -579,13 +594,13 @@ Fixpoint serialize_tree_shape (t : binary_tree unit) :=
   match t with
   | Leaf => Serializer.empty
   | Branch _ b1 b2 =>
-    Serializer.append (serialize "(")
+    Serializer.append (serialize x00)
                       (Serializer.append (serialize_tree_shape b1)
                                          (Serializer.append (serialize_tree_shape b2)
-                                                        (serialize ")")))
+                                                        (serialize x01)))
   end.
 
-Definition serialize_tree_shape_step (b : ascii) (s : bool) :=
+Definition serialize_tree_shape_step (b : byte) (s : bool) :=
   @Error bool (binary_tree unit).
 
 Definition deserialize_tree_shape :=
@@ -603,11 +618,18 @@ Extract Inductive fold_state => "Serializer_primitives.fold_state"
                                   ["Serializer_primitives.Done"
                                      "Serializer_primitives.More"
                                      "Serializer_primitives.Error"].
+
+Extract Inductive byte =>
+"char"
+  ["'\000'" "'\001'" "'\002'" "'\003'" "'\004'" "'\005'" "'\006'" "'\007'" "'\008'" "'\009'" "'\010'" "'\011'" "'\012'" "'\013'" "'\014'" "'\015'" "'\016'" "'\017'" "'\018'" "'\019'" "'\020'" "'\021'" "'\022'" "'\023'" "'\024'" "'\025'" "'\026'" "'\027'" "'\028'" "'\029'" "'\030'" "'\031'" "'\032'" "'\033'" "'\034'" "'\035'" "'\036'" "'\037'" "'\038'" "'\039'" "'\040'" "'\041'" "'\042'" "'\043'" "'\044'" "'\045'" "'\046'" "'\047'" "'\048'" "'\049'" "'\050'" "'\051'" "'\052'" "'\053'" "'\054'" "'\055'" "'\056'" "'\057'" "'\058'" "'\059'" "'\060'" "'\061'" "'\062'" "'\063'" "'\064'" "'\065'" "'\066'" "'\067'" "'\068'" "'\069'" "'\070'" "'\071'" "'\072'" "'\073'" "'\074'" "'\075'" "'\076'" "'\077'" "'\078'" "'\079'" "'\080'" "'\081'" "'\082'" "'\083'" "'\084'" "'\085'" "'\086'" "'\087'" "'\088'" "'\089'" "'\090'" "'\091'" "'\092'" "'\093'" "'\094'" "'\095'" "'\096'" "'\097'" "'\098'" "'\099'" "'\100'" "'\101'" "'\102'" "'\103'" "'\104'" "'\105'" "'\106'" "'\107'" "'\108'" "'\109'" "'\110'" "'\111'" "'\112'" "'\113'" "'\114'" "'\115'" "'\116'" "'\117'" "'\118'" "'\119'" "'\120'" "'\121'" "'\122'" "'\123'" "'\124'" "'\125'" "'\126'" "'\127'" "'\128'" "'\129'" "'\130'" "'\131'" "'\132'" "'\133'" "'\134'" "'\135'" "'\136'" "'\137'" "'\138'" "'\139'" "'\140'" "'\141'" "'\142'" "'\143'" "'\144'" "'\145'" "'\146'" "'\147'" "'\148'" "'\149'" "'\150'" "'\151'" "'\152'" "'\153'" "'\154'" "'\155'" "'\156'" "'\157'" "'\158'" "'\159'" "'\160'" "'\161'" "'\162'" "'\163'" "'\164'" "'\165'" "'\166'" "'\167'" "'\168'" "'\169'" "'\170'" "'\171'" "'\172'" "'\173'" "'\174'" "'\175'" "'\176'" "'\177'" "'\178'" "'\179'" "'\180'" "'\181'" "'\182'" "'\183'" "'\184'" "'\185'" "'\186'" "'\187'" "'\188'" "'\189'" "'\190'" "'\191'" "'\192'" "'\193'" "'\194'" "'\195'" "'\196'" "'\197'" "'\198'" "'\199'" "'\200'" "'\201'" "'\202'" "'\203'" "'\204'" "'\205'" "'\206'" "'\207'" "'\208'" "'\209'" "'\210'" "'\211'" "'\212'" "'\213'" "'\214'" "'\215'" "'\216'" "'\217'" "'\218'" "'\219'" "'\220'" "'\221'" "'\222'" "'\223'" "'\224'" "'\225'" "'\226'" "'\227'" "'\228'" "'\229'" "'\230'" "'\231'" "'\232'" "'\233'" "'\234'" "'\235'" "'\236'" "'\237'" "'\238'" "'\239'" "'\240'" "'\241'" "'\242'" "'\243'" "'\244'" "'\245'" "'\246'" "'\247'" "'\248'" "'\249'" "'\250'" "'\251'" "'\252'" "'\253'" "'\254'" "'\255'" ].
+
 Extract Inlined Constant Serializer.putByte => "Serializer_primitives.putByte".
 Extract Inlined Constant Serializer.empty => "Serializer_primitives.empty".
 Extract Inlined Constant Serializer.append => "Serializer_primitives.append".
-Extract Inlined Constant Deserializer.bind => "Serializer_primitives.bind".
+
 Extract Inlined Constant Deserializer.getByte => "Serializer_primitives.getByte".
+Extract Inlined Constant Deserializer.bind => "Serializer_primitives.bind".
+Extract Inlined Constant Deserializer.fail => "Serializer_primitives.fail".
 Extract Inlined Constant Deserializer.map => "Serializer_primitives.map".
 Extract Inlined Constant Deserializer.ret => "Serializer_primitives.ret".
 Extract Inlined Constant Deserializer.fold => "Serializer_primitives.fold".
